Spec# added to comparison and displace verified in Dafny

Frama-C/append.c
@@ -1,10 +1,11 @@
 #include <stdio.h>
 #include <stdlib.h>
-
+#include "include.h"
 // Append a single item onto the end of the array
 /*@ requires 0 < len < 2147483646;
   @ requires \valid( items+ (0..(len - 1) ) );
-  @ assigns \nothing;
+  @ requires \valid( item );
+  @ assigns result;
   @ ensures \forall integer k; 0 <= k < len ==> \result[k] == items[k];
   @ ensures \result[len] == item;
   @*/
@@ -12,7 +13,7 @@ int* append ( int* items, const int len, const int item )
 {
   // The goal is to implement, specify and verify this function!
   int result[] = malloc ( ( len + 1 ) * sizeof ( int ) );
-  /*@ loop assigns i, result[i];
+  /*@ loop assigns i, result[0..(i-1)];
     @ loop invariant \forall integer k; 0 <= k < i ==> items[k] == result[k];
     @ loop variant len - i; */
   for ( int i = 0; i < len; ++i )
@@ -20,33 +21,6 @@ int* append ( int* items, const int len, const int item )
   result[len] = item;
   free( items );
   return result;
-}
-
-/*@ requires len > 0;
-  @ requires \valid( items+ ( 0..(len - 1) ) );
-  @ assigns items[0..(len - 1)];
-  @ ensures \valid( items+ ( 0..(len - 1) ) );
-  @ ensures \forall integer k; 0 <= k < len ==> items[k] == k;
-  */
-void fillarr ( int* items, const int len )
-{
-  /*@ loop assigns i, items[i];
-    @ loop invariant \forall integer k; 0 <= k < i ==> items[k] == k;
-    @ loop variant len - i; */
-  for ( int i = 0; i < len; ++i )
-    items[i] = i;
-}
-
-/*@ requires len > 0;
-  @ assigns \nothing; */
-void printarr ( int* items, const int len )
-{
-  printf ( "array = [ " );
-  /*@ loop assigns i;
-    @ loop variant len - i; */
-  for ( int i = 0; i < len - 1; i++ )
-    printf ( "%d ,", items[i] );
-  printf ( len > 0 ? "%d ]\n" : "]\n", items[len - 1] );
 }
 
 int main()
