Frama-C/copy.c
@@ -1,34 +1,14 @@
-#include <stdio.h>
-#include <stdlib.h>
+#include "copy.h"
 
-/*  Starting points in both arrays cannot be negative.
-    Source array must contain enough elements to be copied.
-    Destination array must have enough space for copied elements.
-    Result is same size as dest.
-    All elements before copied region are same.
-    All elements in copied region match src.
-    All elements above copied region are same.
-  */
-/*@ requires sStart >= 0;
-  @ requires dStart >= 0;
-  @ requires range > 0;
-  @ requires slen >= sStart + range;
-  @ requires dlen >= dStart + range;
-  @ requires \separated( src+ (0..(slen - 1) ), dest+ (0..(dlen - 1) ) );
-  @ requires \valid( src+ (0..(slen - 1) ) );
-  @ requires \valid( dest+ (0..(dlen - 1) ) );
-  @ assigns dest[dStart..(dStart + range)];
-  @ ensures \forall integer k; 0 <= k < range ==> dest[dStart + k] == src[sStart + k];
-  */
-void copy( const int src[], const size_t slen, const size_t sStart
-              , int dest[], const size_t dlen, const size_t dStart, const size_t range )
+void copy( const int src[], const int slen, const int sStart
+              , int dest[], const int dlen, const int dStart, const int range )
 {
-  size_t i = 0;
+  int i = 0;
   /*All items are still the same before dStart index.
     All items after dStart index are still the same.
     Inbetween items are copied from src.
     */
-  /*@ loop assigns i, dest[dStart..(dStart + i)];
+  /*@ loop assigns i, dest[dStart..(dStart + i - 1)];
     @ loop invariant 0 <= i <= range;
     @ loop invariant \forall integer k; 0 <= k < i ==> src[sStart + k] == dest[dStart + k];
     @ loop variant range - i;
@@ -40,37 +20,3 @@ void copy( const int src[], const size_t slen, const size_t sStart
   }
 }
 
-/*@ requires len > 0;
-  @ requires \valid( items+ ( 0..(len - 1) ) );
-  @ assigns items[0..(len - 1)];
-  @ ensures \forall integer k; 0 <= k < len ==> items[k] == k;
-  */
-void fillarr( int* items, size_t len )
-{
-  /*@ loop assigns i, items[0..(i - 1)];
-    @ loop invariant \forall integer k; 0 <= k < i ==> items[k] == k;
-    @ loop variant len - i; */
-  for ( int i = 0; i < len; ++i )
-    items[i] = i;
-}
-
-/*@ requires len > 0;
-  @ assigns \nothing; */
-void printarr( int* items, size_t len )
-{
-  printf( "array = [ " );
-  /*@ loop assigns i;
-    @ loop variant len - i; */
-  for(int i = 0; i < len - 1; i++)
-    printf( "%d ,", items[i] );
-  printf( len > 0 ? "%d ]\n" : "]\n", items[len - 1] );
-}
-
-int main()
-{
-  int src[] = { 6, 7, 8, 9, 10 };
-  int res[] = malloc( 5 * sizeof(int) );
-  fillarr( res, 5 );
-  copy( src, 5, 1, res, 5, 1, 3 );
-  printarr( res, 5 );
-}
