Frama-C/copy.h
@@ -1,0 +1,26 @@
+#ifndef COPY_H_INCLUDED
+#define COPY_H_INCLUDED
+
+#include <stdio.h>
+
+/*@
+  // Starting points in both arrays cannot be negative.
+  @ requires sStart >= 0;
+  @ requires dStart >= 0;
+  // Source array must contain enough elements to be copied.
+  @ requires range > 0;
+  // Destination array must have enough space for copied elements.
+  @ requires slen >= sStart + range;
+  @ requires dlen >= dStart + range;
+  @ requires \separated( src+ (0..(slen - 1) ), dest+ (0..(dlen - 1) ) );
+  @ requires \valid( src+ (0..(slen - 1) ) );
+  @ requires \valid( dest+ (0..(dlen - 1) ) );
+  // All elements before and after the copied region are same.
+  @ assigns dest[dStart..(dStart + range)];
+  // All elements in copied region match src.
+  @ ensures \forall integer k; 0 <= k < range ==> dest[dStart + k] == src[sStart + k];
+  */
+void copy( const int src[], const int slen, const int sStart
+              , int dest[], const int dlen, const int dStart, const int range );
+
+#endif // COPY_H_INCLUDED
