Frama-C/include.c
@@ -1,0 +1,20 @@
+#include "include.h"
+
+void fillarr( int* items, size_t len )
+{
+  /*@ loop assigns i, items[0..(i - 1)];
+    @ loop invariant \forall integer k; 0 <= k < i ==> items[k] == k;
+    @ loop variant len - i; */
+  for ( int i = 0; i < len; ++i )
+    items[i] = i;
+}
+
+void printarr( int* items, size_t len )
+{
+  printf( "array = [ " );
+  /*@ loop assigns i;
+    @ loop variant len - i; */
+  for(int i = 0; i < len - 1; i++)
+    printf( "%d ,", items[i] );
+  printf( len > 0 ? "%d ]\n" : "]\n", items[len - 1] );
+}
