Frama-C/include.h
@@ -1,0 +1,20 @@
+#ifndef INCLUDE_H_INCLUDED
+#define INCLUDE_H_INCLUDED
+
+#include <stdio.h>
+
+/*@ requires len > 0;
+  @ requires items != \null;
+  @ requires \valid_range( items, 0, len - 1 );
+  @ assigns items[0..(len - 1)];
+  @ ensures \forall integer k; 0 <= k < len ==> items[k] == k;
+  */
+void fillarr( int* items, size_t len );
+
+/*@ requires len > 0;
+  @ requires items != \null;
+  @ requires \valid_range( items, 0, len - 1 );
+  @ assigns \nothing; */
+void printarr( int* items, size_t len );
+
+#endif // INCLUDE_H_INCLUDED
