Dafny/alt/displace.dfy
@@ -1,28 +1,60 @@
-// Status: verifies and compiles
-// rotates a region of the array by one place backward
-method displace(arr: array<int>, start: nat, len: nat)
-  modifies arr
+// Status: verifier infinite loop
+// rotates a region of the array by one place forward
+
+predicate rotated(o:seq<int>, r:seq<int>) 
+  requires |o| == |r|
+{
+  (forall i :: 1 <= i < |o| ==> r[i] == o[i-1]) &&
+  (|o| > 0 ==> r[0] == o[|o|-1])  
+}
+
+method displace(arr: array<int>, start: nat, len: nat) returns (r: array<int>)
   requires arr != null
   requires start + len <= arr.Length
-  //
-  ensures arr != null && arr.Length == old(arr.Length)
-  ensures forall k: nat :: k < start ==> arr[k] == old(arr[k])
-  ensures forall k: nat :: (start + len) <= k < arr.Length ==> arr[k] == old(arr[k])
-  ensures forall k :: start <= k < (start + len)
-                 ==> arr[start + (((k + 1) - start) % len)] == old(arr[k])
+  ensures r != null && r.Length == arr.Length
+  ensures arr[..start] == r[..start]
+  ensures arr[(start + len)..] == r[(start + len)..]
+  ensures rotated(arr[start .. start+len], r[start .. start+len])
 {
-  var i := start + len - 2;
-  var temp := arr[start + len - 1];
+  var i: nat := 0;
+  r := new int[arr.Length];
+  while i < start
+    invariant i <= start
+    invariant forall k: nat :: k < i ==> r[k] == arr[k]
+    {
+      r[i] := arr[i];
+      i := i + 1;
+    }
+    
+    assert arr[..start] == r[..start];
   
-  while i >= start
-    invariant start <= i <= (start + len)
-    invariant arr[..start] == old(arr[..start])
-    invariant forall k :: start <= k < i
-              ==> arr[start + (((k + 1) - start) % len)] == old(arr[k])
-    invariant arr[(start + len)..] == old(arr[(start + len)..])
-  {
-      arr[i + 1] := arr[i];
-      i := i - 1;
+  if len > 0 {
+    r[start] := arr[start+len-1];
+    
+    assert r[start] == arr[start+len-1];
+    
+    i := start+1;
+    while i < start+len
+      invariant start < i <= start+len
+      invariant arr[..start] == r[..start]
+      invariant r[start] == arr[start+len-1]
+      invariant forall k: nat :: start < k < i ==> r[k] == arr[k-1]
+      {
+        r[i] := arr[i-1];
+        i := i + 1;
+      }
   }
-  arr[start] := temp;
+  
+  assert rotated(arr[start .. start+len], r[start .. start+len]);
+  
+  i := start+len;
+  while i < arr.Length
+    invariant start+len <= i <= arr.Length
+    invariant arr[..start] == r[..start]
+    invariant rotated(arr[start .. start+len], r[start .. start+len])
+    invariant forall k: nat :: start+len <= k < i ==> r[k] == arr[k]
+    {
+      r[i] := arr[i];
+      i := i + 1;
+    }
 }
