Dafny/displace.dfy
@@ -1,7 +1,16 @@
 // Status: verifier infinite loop
+
+predicate rotated(o:seq<int>, r:seq<int>) 
+requires |o| == |r|
+{
+  (forall i :: 1 <= i < |o| ==> r[i] == o[i-1]) &&
+  (|o| > 0 ==> r[0] == o[|o|-1])  
+}
+
 // rotates a region of the array by one place forward
 method displace(arr: array<int>, start: nat, len: nat) returns (r: array<int>)
   requires arr != null
+  requires len > 1
   requires start + len <= arr.Length
   // returned array is the same size as input arr
   ensures r != null && r.Length == arr.Length
@@ -9,31 +18,36 @@ method displace(arr: array<int>, start: nat, len: nat) returns (r: array<int>)
   ensures arr[..start] == r[..start]
   // elements after the end of the rhe region are unchanged
   ensures arr[(start + len)..] == r[(start + len)..]
-  // elements in the region are skewed by one in a positive direction and wrap around
-  ensures forall k :: start <= k < (start + len)
-                 ==> r[start + (((k + 1) - start) % len)] == arr[k]
+  // elements in the region are skewed by one in a positive direction and wrap
+  // around
+  ensures rotated(arr[start .. start+len], r[start .. start+len])
 {
-    var i: nat := 0;
-    r := new int[arr.Length];
-    
-    while i < arr.Length
-      invariant i <= arr.Length
-      invariant forall k: nat :: k < i ==> r[k] == arr[k]
-    {
-        r[i] := arr[i];
-        i := i + 1;
-    }
-    
-    i := start;
-    
-    while i < (start + len)
-      invariant start <= i <= (start + len)
-      invariant arr[..start] == r[..start]
-      invariant arr[(start + len)..] == r[(start + len)..]
-      invariant forall k :: start <= k < i
-                ==> r[start + (((k + 1) - start) % len)] == arr[k]
-    {
-        r[start + (((i + 1) - start) % len)] := arr[i];
-        i := i + 1;
-    }
+  var i: nat := 0;
+  r := new int[arr.Length];
+  
+  // just copy the array
+  while i < arr.Length
+    invariant i <= arr.Length
+    invariant forall k: nat :: k < i ==> r[k] == arr[k]
+  {
+    r[i] := arr[i];
+    i := i + 1;
+  }
+  assert arr[..start] == r[..start] && arr[(start + len)..] == r[(start + len)..];
+  
+  i := 1;
+  r[start] := arr[start + len - 1];
+  
+  // rotate the array region between start to len
+  while i < len
+    invariant 0 < i <= len
+    invariant r[..start] == arr[..start]
+    invariant r[start] == arr[start + len - 1]
+    invariant r[(start + len)..] == arr[(start + len)..]
+    invariant forall k :: 0 < k < i ==> r[start + k] == arr[start + k - 1]
+  {
+    r[start + i] := arr[start + i - 1];
+    i := i + 1;
+  }
+  assert rotated(arr[start .. start+len], r[start .. start+len]);
 }
