Dafny/alt/displaceInPlace.dfy
@@ -1,0 +1,36 @@
+// Status: verifier infinite loop
+// rotates a region of the array by one place forward
+method displace(arr: array<int>, start: nat, len: nat)
+  requires arr != null
+  requires len > 1
+  requires start + len <= arr.Length
+  modifies arr;
+  // returned array is the same size as input arr
+  ensures arr != null && arr.Length == old(arr.Length)
+  // elements before the start of the region are unchanged
+  ensures arr[..start] == old(arr[..start])
+  // elements after the end of the rhe region are unchanged
+  ensures arr[(start + len)..] == old(arr[(start + len)..])
+  // elements in the region are skewed by one in a positive direction and wrap
+  // around
+  ensures forall k :: 0 < k < len
+                 ==> arr[start + k] == old(arr[start + k - 1])
+  ensures arr[start] == old(arr[start + len - 1])
+{
+  var i: nat := len - 1;
+  var temp := arr[start + i]; // end of region element
+  
+  // rotate the region
+  while i > 0
+    invariant 0 <= i < len
+    invariant arr[..start] == old(arr[..start])
+    invariant arr[(start + len)..] == old(arr[(start + len)..])
+    invariant forall k :: i < k < len 
+              ==> arr[start + k] == old(arr[start + k - 1])
+  {
+    arr[start + i] := arr[start + i - 1];
+    i := i - 1;
+  }
+  
+  arr[start] := temp;
+}
