Dafny/binarySearch.dfy
@@ -1,15 +1,18 @@
+// Status: verifies and compiles
 predicate sorted(s: seq<int>)
 {
    forall i,j :: 0 <= i < j < |s| ==> s[i] <= s[j]
 }
 
-method BinarySearch(a: array<int>, key: int) returns (index: int)    
+method BinarySearch(a: array<int>, key: int) returns (index: int)  
+  
   requires a != null && sorted(a[..])
   ensures index >= 0 ==> index < a.Length && a[index] == key
   ensures index < 0  ==> forall k: nat :: k < a.Length ==> a[k] != key
 {
   var low := 0;
-  var high := a.Length;       
+  var high := a.Length;     
+  
 
   while (low < high)
     invariant 0 <= low <= high <= a.Length
@@ -27,7 +30,10 @@ method BinarySearch(a: array<int>, key: int) returns (index: int)
       else
       {
           return mid;
-      }       
-  }       
+      }     
+  
+  }     
+  
   return -1;
-}        
+}       
+ 
