Dafny/find.dfy
@@ -1,3 +1,4 @@
+// Status: verifies and compiles
 predicate sorted(s: seq<int>)
 {
   forall i,j :: 0 <= i < j < |s| ==> s[i] <= s[j]
