binarySearch.whiley
@@ -1,0 +1,35 @@
+// Status: verifies and compiles?...no
+//         ( if a[mid] < key:, index out of bounds (negative) )
+// Search through a sorted list by way of narrowing the search by half upon
+// each iteration. rerturns the index of item or -1 if not found
+type nat is (int n) where n >= 0
+
+method BinarySearch( int[] a, int key ) -> (int r)  
+//////////////////////////////////////////////////
+requires all { i in 0..|a|, j in 0..|a| | i <= j ==> a[i] <= a[j] }
+ensures r >= 0 ==> r < |a| && a[r] == key
+ensures r < 0  ==> all { k in 0..|a| | a[k] != key }
+:
+  nat low = 0
+  nat high = |a|
+  nat mid = 0
+
+  while low < high
+  ////////////////
+  where high <= |a|
+  where  low <= |a|
+  where  mid <= |a|
+  where  low <= high 
+  where  low <= mid
+  where  mid <= high
+  // elements outside the search range are not eqaul to key
+  where all { i in 0..|a| | !(low <= i && i < high) ==> a[i] != key }
+  :
+    mid = (low + high) / 2
+    if a[mid] < key:
+      low = mid + 1
+    else if key < a[mid]:
+      high = mid
+    else:
+      return mid
+  return -1
