displace.whiley
@@ -1,13 +1,13 @@
-// Status wyc-37: loop invariant does not hold on entry [1192ms]
-//                where all { k in start..i | result[k] ==
-//                          arr[start + (((k + 1) - start) % len)] }
-//                (i == start on entry) --> start..start is empty.
-//        wyc-36: verification infinite loop
+// Status wyc-37: verification infinite loop
+//        wyc-36: loop invariant not restored [1192ms]
+//                where all { k in 0 .. start | result[k] == arr[k] }
+//        
 type nat is (int n) where n >= 0
 
 // rotates a region of the array by one place forward
 function displace(int[] arr, nat start, nat len) -> (int[] r)
 /////////////////////////////////////////////////////////////
+requires len > 1
 requires start + len <= |arr|
 // output array is the same size as input array
 ensures |r| == |arr|
@@ -16,23 +16,25 @@ ensures all { k in 0..start | r[k] == arr[k] }
 // all elements after the region remain the same
 ensures all { k in (start + len)..|arr| | r[k] == arr[k] }
 // all elements in the region are rotated by one place
-ensures all { k in start..start + len | r[k] == arr[start + (((k + 1) - start) % len)] }
+ensures all { k in start + 1..start + len | r[k] == arr[k - 1] }
+ensures r[start] == arr[start + len - 1]
 :
-  nat i = start
+  nat i = start + 1
   int[] result = arr
-  assert all { k in 0..|result| | result[k] == arr[k] }
+  assume all { k in 0..|result| | result[k] == arr[k] }
 
   while i < (start + len)
-
-  where start <= i where i <= (start + len)
+  ///////////////////////
+  where start < i where i <= (start + len)
   where |result| == |arr|
-  where all { k in 0..start | result[k] == arr[k] }
-  where all { k in start..i | result[k] == arr[start + (((k + 1) - start) % len)] }
-  where all { k in (start + len)..|arr| | result[k] == arr[k] }
+  where all { k in          0 .. start + 1 | result[k] == arr[k] }
+  where all { k in  start + 1 .. i         | result[k] == arr[k - 1] }
+  where all { k in (start+len)..|arr|      | result[k] == arr[k] }
   :
-    result[i] = arr[start + (((i + 1) - start) % len)]
+    result[i] = arr[i - 1]
     i = i + 1
 
   assert i == (start + len)
+  result[start] = arr[start + len - 1]
   
   return result
